fixed some problems with the caching example

examples/relational/cache.fst
@@ -1,5 +1,5 @@
 (*--build-config
-    options:--admit_fsi Set;
+    options:--admit_fsi Set --z3timeout 15;
     variables:LIB=../../lib;
     other-files:$LIB/set.fsi $LIB/heap.fst $LIB/st.fst $LIB/all.fst $LIB/st2.fst $LIB/list.fst
   --*)
@@ -8,8 +8,8 @@ module Cache
 
 open Relational
 open Comp
-open Heap
 open List
+open Heap
 
 (* Functional Sepcification of Factorials *)
 val fac : nat -> Tot nat
@@ -17,26 +17,32 @@ let rec fac x = if x = 0 then 1 else  fac (x-1) * x
 
 (* A tail-recursive imperative implementation *)
 val imp_fac : x:ref nat -> a:ref nat 
-  -> ST nat (requires (fun h -> a <> x))
+  -> ST nat (requires (fun h -> a <> x 
+                             /\ contains h a 
+                             /\ contains h x ))
             (ensures  (fun h r h' -> a <> x 
                                   /\ r = (fac (sel h x) * (sel h a))
                                   /\ sel h' x = 0 
                                   /\ sel h' a = r
-                                  /\ modifies (a ^+^ x) h h'))
+                                  /\ equal h' (upd (upd h x 0) a r)))
 let rec imp_fac x a = 
   if !x = 0 then 
     !a 
   else 
   ( a := !a * !x;
-    x := !x -1;
-    imp_fac x a)
+    x := !x - 1;
+    imp_fac x a 
+    )
+
 
 (* A wrapper for the recursive function, ensuring that the heap will not be
    modified *)
 val imp_fac_wrap : x:ref nat -> a:ref nat -> y:nat 
-  -> ST nat (requires  (fun h -> a <> x))
+  -> ST nat (requires  (fun h -> a <> x
+                              /\ contains h a 
+                              /\ contains h x ))
             (ensures   (fun h r h' -> r = fac y 
-                                       /\ modifies Set.empty h h'))
+                                   /\ equal h h'))
 let imp_fac_wrap x a y =
   let tmp1 = !x in 
   let tmp2 = !a in
@@ -54,9 +60,10 @@ assume val cache : ref fac_cache
 type fac_cache_correct (c:fac_cache) = (forall x. is_Some (assoc x c) ==> (Some.v (assoc x c) = fac x))
 
 (* A cached version of the factorial computation *)
-val fac_cached : x:nat -> ST nat (requires (fun h -> fac_cache_correct (sel h cache)))
+val fac_cached : x:nat -> ST nat (requires (fun h -> fac_cache_correct (sel h cache)
+                                                  /\ contains h cache))
                                  (ensures  (fun h r h' ->  fac_cache_correct (sel h' cache)
-                                                        /\ modifies (only cache) h h'
+                                                        /\ (exists c. equal h' (upd h cache c))
                                                         /\ r = fac x))
 let fac_cached x =
   let c = !cache in
@@ -68,25 +75,16 @@ let fac_cached x =
     cache := (x,v) :: c;
     fac x)
 
-(* Can we maybe proof this? (modifies is defined based on equality..) *)
-(* Maybe it is also better to define an own predicate for this, because we are
-   somehow "abusing" modifies for a different purpose *)
-assume val heap_modifies_refl : h0:heap -> h1:heap -> mods:Set.set Heap.aref
-  -> Lemma (requires (modifies mods h0 h1))
-           (ensures  (modifies mods h1 h0))
-(* let heap_modifies_refl h0 h1 mods = () *)
-
 (* Proof that the functions compute the same values and that cache is the only
-   memory cell that can be modified *)
+   memory cell that can be different in the two runs *)
 val correct : x:ref nat -> a:ref nat -> y:eq nat
   -> ST2 (eq nat)
          (requires (fun h -> fac_cache_correct (sel (R.r h) cache)
                           /\ x <> a 
-                          /\ modifies (only cache) (R.l h) (R.r h)))
+                          /\ contains (R.l h) x 
+                          /\ contains (R.l h) a 
+                          /\ contains (R.r h) cache
+                          /\ (exists c. equal (upd (R.l h) cache c) (R.r h))))
          (ensures (fun h _ h' -> fac_cache_correct (sel (R.r h') cache)
-                              /\ modifies (only cache) (R.l h') (R.r h')))
-let correct x a y =   let h = compose2_self ST.get (twice ()) in 
-                      let res = compose2 (fun y -> imp_fac_wrap x a y) (fun x -> fac_cached x) y in
-                      let h' = compose2_self ST.get (twice ()) in 
-                      heap_modifies_refl (R.l h) (R.l h') (Set.empty);
-                      res
+                              /\ (exists c. equal (upd (R.l h') cache c) (R.r h'))))
+let correct x a y =   compose2 (fun y -> imp_fac_wrap x a y) (fun x -> fac_cached x) y 
